Speed-up compilation of TableauxRocq proofs (#12)
This PR addresses issue #2, and changes TableauxRocq to make its base
structure more focused towards computations. Now, most of the
development uses *reflection*, i.e., boolean equality with completeness
w.r.t. the propositional equality. This enables us to vastly simplify
the `set_decide` tactic, and actually remove it altogether. Indeed, as
everything is setup to compute efficiently, it now suffices to use
`native_compute` (or `vm_compute`) to decide those goals instead of
doing heavy rewrites and using decision tactics.

This already provides an important speedup in the first small
perfromance test `perfs_1.v`, that compiles in approximately 2.65s on my
machine on the `master` branch, when it compiles in 0.5s after this PR.

As the boolean equality we assume is complete, it does not impedes
proofs which can proceed as was the case before modulo a small rewrite.

I also provide a script that automatically benches the proposed changes
w.r.t. the commit that diverges from master, and integrate it into the
CI after the building of the library succeeds.

Note that some constructs are still not computing properly (which makes
it impossible e.g. to finish a `hasTableau` proof by `now esimpl`), but
most of the important ones are.

Issue #2 has been updated in consequence.

theories/Prelude/Sets.v
@@ -8,25 +8,31 @@ From Stdlib Require Import MSets.MSetProperties.
 From Stdlib Require Import MSets.MSetFacts.
 From Stdlib Require Import MSets.MSetDecide.
 
+Create HintDb set_db.
+
 (** ** Axiomatization of sets as a typeclass *)
 Class set {A : Type} :=
   { car :> Type
 
+  ; set_eqb :: EqBool car
+
   (** *** Basic set operations *)
   ; empty_set : car
-  ; mem : A -> car -> Prop
+  ; mem : A -> car -> bool       (** Use [mem] in definitions to compute *)
+  ; set_in : A -> car -> Prop    (** Use [mem_spec] to convert [mem] to [set_in] in proofs *)
   ; union : car -> car -> car
   ; inter : car -> car -> car
   ; singleton : A -> car
 
   (** *** Extensionality property of sets *)
-  ; set_ext : forall (s1 s2 : car), s1 = s2 <-> (forall (x : A), mem x s1 <-> mem x s2)
+  ; set_ext : forall (s1 s2 : car), s1 = s2 <-> (forall (x : A), set_in x s1 <-> set_in x s2)
 
   (** *** Properties of defined operations *)
-  ; empty_spec : forall (x : A), mem x empty_set -> False
-  ; singleton_spec : forall (x y : A), mem x (singleton y) <-> x = y
-  ; union_spec : forall (x : A) (s1 s2 : car), mem x (union s1 s2) <-> mem x s1 \/ mem x s2
-  ; inter_spec : forall (x : A) (s1 s2 : car), mem x (inter s1 s2) <-> mem x s1 /\ mem x s2 }.
+  ; empty_spec : forall (x : A), set_in x empty_set -> False
+  ; mem_spec : forall (x : A) (s : car), mem x s = true <-> set_in x s
+  ; singleton_spec : forall (x y : A), set_in x (singleton y) <-> x = y
+  ; union_spec : forall (x : A) (s1 s2 : car), set_in x (union s1 s2) <-> set_in x s1 \/ set_in x s2
+  ; inter_spec : forall (x : A) (s1 s2 : car), set_in x (inter s1 s2) <-> set_in x s1 /\ set_in x s2 }.
 Arguments set : clear implicits.
 
 Notation "S1 \union S2" := (union S1 S2) (at level 30).
@@ -40,21 +46,21 @@ Section SetProperties.
 
   Lemma add_spec1 :
     forall (x : A) (s : set_A),
-      mem x (add x s).
+      set_in x (add x s).
   Proof using Type.
     intros x s; unfold add. rewrite union_spec. left. rewrite singleton_spec. reflexivity.
   Qed.
 
   Lemma add_spec2 :
     forall (x y : A) (s : set_A),
-      mem x s -> mem x (add y s).
+      set_in x s -> set_in x (add y s).
   Proof using Type.
     intros x y s hin; unfold add. rewrite union_spec. now right.
   Qed.
 
   Lemma add_inv :
     forall (x y : A) (s : set_A),
-      mem x (add y s) -> x = y \/ mem x s.
+      set_in x (add y s) -> x = y \/ set_in x s.
   Proof using Type.
     intros ??? hin. rewrite /add union_spec in hin. destruct hin as [hin | hin].
     - rewrite singleton_spec in hin. now left.
@@ -72,7 +78,7 @@ Section SetProperties.
   Qed.
 
   Definition subset (s1 s2 : set_A) :=
-    forall (x : A), mem x s1 -> mem x s2.
+    forall (x : A), set_in x s1 -> set_in x s2.
 
   #[global] Instance reflexive_subset : Reflexive subset.
   Proof using Type. intro. unfold subset. tauto. Qed.
@@ -87,7 +93,7 @@ Section SetProperties.
 
   Lemma is_empty_spec :
     forall (x : A) (s : set_A),
-      is_empty s -> mem x s -> False.
+      is_empty s -> set_in x s -> False.
   Proof using Type. intros ?? e. rewrite e. apply empty_spec. Qed.
 
   Lemma empty_is_empty :
@@ -96,7 +102,7 @@ Section SetProperties.
 
   Lemma is_empty_spec' :
     forall (s : set_A),
-      (forall (x : A), mem x s -> False) -> is_empty s.
+      (forall (x : A), set_in x s -> False) -> is_empty s.
   Proof using Type.
     intros. have e : s = empty_set.
     { apply set_ext; intro y; cbn. split.
@@ -129,12 +135,12 @@ Section SetProperties.
 
   Lemma mem_unionl :
     forall (x : A) (s1 s2 : set_A),
-      mem x s1 -> mem x (union s1 s2).
+      set_in x s1 -> set_in x (union s1 s2).
   Proof using Type. intros. rewrite union_spec. now left. Qed.
 
   Lemma mem_unionr :
     forall (x : A) (s1 s2 : set_A),
-      mem x s2 -> mem x (union s1 s2).
+      set_in x s2 -> set_in x (union s1 s2).
   Proof using Type. intros. rewrite union_spec. now right. Qed.
 
   Lemma empty_unitl :
@@ -181,6 +187,7 @@ Section SetProperties.
     intros; apply set_ext; intro; split; intro hin; rewrite !union_spec in hin |- *;
       destruct hin as [hin | hin]; try destruct hin as [hin | hin]; firstorder.
   Qed.
+  Hint Rewrite empty_unitl empty_unitr union_idemp union_assoc : set_db.
 
   Lemma inter_sym :
     forall (s1 s2 : set_A), inter s1 s2 = inter s2 s1.
@@ -189,11 +196,22 @@ Section SetProperties.
       firstorder.
   Qed.
 
-  Definition disjoint (s1 s2 : set_A) := inter s1 s2 = empty_set.
+  Definition disjoint (s1 s2 : set_A) := Classes.eqb (s1 \inter s2) empty_set.
+  Definition are_disjoint (s1 s2 : set_A) := s1 \inter s2 = empty_set.
+  Hint Unfold are_disjoint : set_db.
+
+  Lemma disjoint_are_disjoint :
+    forall (s1 s2 : set_A),
+      disjoint s1 s2 = true <-> are_disjoint s1 s2.
+  Proof using Type.
+    intros. transitivity (forall (x : A), set_in x (s1 \inter s2) <-> set_in x empty_set).
+    - rewrite eqbIsEq. apply set_ext.
+    - symmetry. apply set_ext.
+  Qed.
 
   Lemma empty_disjointl :
     forall (s : set_A),
-      disjoint empty_set s.
+      are_disjoint empty_set s.
   Proof using Type.
     intro s. apply set_ext; intro; split; intro hin.
     - now rewrite inter_spec in hin.
@@ -202,14 +220,14 @@ Section SetProperties.
 
   Lemma empty_disjointr :
     forall (s : set_A),
-      disjoint s empty_set.
-  Proof using Type. intro; unfold disjoint. rewrite inter_sym. apply empty_disjointl. Qed.
+      are_disjoint s empty_set.
+  Proof using Type. intro; autounfold with set_db. rewrite inter_sym. apply empty_disjointl. Qed.
 
   Lemma disjoint_sym :
     forall (s1 s2 : set_A),
-      disjoint s1 s2 <-> disjoint s2 s1.
+      are_disjoint s1 s2 <-> are_disjoint s2 s1.
   Proof using Type.
-    intros s1 s2; unfold disjoint. split; intro e;
+    intros s1 s2; autounfold with set_db. split; intro e;
       now rewrite inter_sym.
   Qed.
 
@@ -218,23 +236,17 @@ Section SetProperties.
       (fold_left (fun (s : set_A) (b : B) => union s (f b)) l s) =
         s \union (fold_left (fun (s : set_A) (b : B) => union s (f b)) l empty_set).
   Proof using Type.
-    intros???; induction l as [|y ys IHys]; intros; cbn in *.
-    - now rewrite empty_unitr.
-    - rewrite empty_unitl. rewrite IHys; cbn.
+    intros???; induction l as [|y ys IHys]; intros; cbn in *; autorewrite with set_db.
+    - reflexivity.
+    - rewrite IHys; cbn.
       have e0 : fold_left (fun (s0 : set_A) (b : B) => s0 \union f b) ys (f y) =
                   (f y) \union fold_left (fun (s0 : set_A) (b : B) => s0 \union f b) ys empty_set.
       { apply IHys. }
       rewrite e0 union_assoc //.
   Qed.
-
-  (* TODO: rewrite it with equalities. Maybe this is the thing above? *)
-  Lemma mem_fold_left_cons_unionl :
-    forall {B : Type} (f : B -> set_A) (b : B) (l : list B) (x : A) (s : set_A),
-      mem x (fold_left (fun (s : set_A) (b : B) => union s (f b)) (b :: l) s) <->
-        mem x (union ((fold_left (fun (s : set_A) (b : B) => union s (f b)) l s)) (f b)).
-  Proof.
-    Admitted.
 End SetProperties.
+Hint Rewrite @empty_unitl @empty_unitr @union_idemp @union_assoc : set_db.
+Hint Unfold are_disjoint : set_db.
 
 (** We denote [\{ x, y, ..., z \}] for finite sets *)
 Notation "\{ \}" := empty_set.
@@ -255,11 +267,13 @@ Module SetComputationalInstances.
     Parameter lt_compat : Proper (eq ==> eq ==> iff) lt.
     Parameter compare : t -> t -> comparison.
     Parameter compare_spec : forall (x y : t), CompareSpec (x = y) (lt x y) (lt y x) (compare x y).
-    Parameter eq_dec : EqDec t.
+    Parameter eq_bool : EqBool t.
   End SimpleOrderedType.
 
   (** Generic instantiation of our [set] from an ordered type *)
   Module SetFromOrdered (X : SimpleOrderedType).
+    Existing Instance X.eq_bool.
+
     Module X_ <: OrderedType.
       Definition t := X.t.
       Definition eq (x y : t) := x = y.
@@ -270,7 +284,7 @@ Module SetComputationalInstances.
       Definition lt_compat := X.lt_compat.
       Definition compare := X.compare.
       Definition compare_spec := X.compare_spec.
-      Definition eq_dec := X.eq_dec.
+      Definition eq_dec := eq_dec_from_eq_bool X.t.
     End X_.
 
     Module SetOfX_ := MSetAVL.Make X_.
@@ -326,11 +340,29 @@ Module SetComputationalInstances.
       intros; rewrite SetOfX_.singleton_spec. reflexivity.
     Qed.
 
+    Lemma SetOfX_equal_eq :
+      forall x y : SetOfX_.t, SetOfX_.equal x y = true <-> x = y.
+    Proof.
+      intros; split.
+      - intro heq. apply SetOfXFacts.equal_2 in heq. now rewrite set_equal_is_eq in heq.
+      - intros []. apply SetOfXFacts.equal_1. apply SetOfXProps.equal_refl.
+    Qed.
+
+    Instance SetOfX_EqBool : EqBool SetOfX_.t.
+    Proof.
+      unshelve econstructor.
+      - exact SetOfX_.equal.
+      - exact SetOfX_equal_eq.
+    Defined.
+
     #[global] Instance set_of_ordered : set X.t :=
       {| car := SetOfX_.t
 
+      ;  set_eqb := ltac:(typeclasses eauto)
+
       ;  empty_set := SetOfX_.empty
-      ;  mem := SetOfX_.In
+      ;  mem := SetOfX_.mem
+      ;  set_in := SetOfX_.In
       ;  union := SetOfX_.union
       ;  inter := SetOfX_.inter
       ;  singleton := SetOfX_.singleton
@@ -339,6 +371,7 @@ Module SetComputationalInstances.
 
       ;  empty_spec := SetOfX_empty_spec
       ;  singleton_spec := SetOfX_singleton_spec
+      ;  mem_spec x s := SetOfX_.mem_spec s x
       ;  union_spec x s1 s2 := SetOfX_.union_spec s1 s2 x
       ;  inter_spec x s1 s2 := SetOfX_.inter_spec s1 s2 x |}.
   End SetFromOrdered.
@@ -351,7 +384,7 @@ Module SetComputationalInstances.
     Definition lt_compat := PeanoNat.Nat.lt_compat.
     Definition compare := PeanoNat.Nat.compare.
     Definition compare_spec := PeanoNat.Nat.compare_spec.
-    Definition eq_dec := @eqDec nat _.
+    Definition eq_bool : EqBool nat := ltac:(typeclasses eauto).
   End OrderedNat.
 
   Module SetOfNat_ := SetFromOrdered OrderedNat.
@@ -404,7 +437,7 @@ Module SetComputationalInstances.
         + inversion e.
         + left. rewrite /Ascii.compare BinNat.N.compare_gt_iff // in ea.
     Qed.
-    Definition eq_dec := @eqDec string _.
+    Definition eq_bool : EqBool string := ltac:(typeclasses eauto).
   End OrderedString.
 
   Module SetOfString_ := SetFromOrdered OrderedString.
