devtools/tests/benchs/perfs_1.v
@@ -1,0 +1,39 @@
+From Tableaux Require Import All.
+
+Import ATPCompat.
+
+Definition Axiom0 : EForm :=
+  EAll "X6" (EEx "Y4" (EPred "p" [(EVar "X6") ; (EVar "Y4")])).
+
+Definition T : EForm :=
+  EAll "X10" (EEx "Y8" (EPred "p" [(EVar "X10") ; (EVar "Y8")])).
+
+Definition subst :=
+  translate_substitution
+    [("Y8_17", (EFun "skolem@Y4@1" [(EFun "skolem@X10@0" [])])); ("X6_13", (EFun "skolem@X10@0" []))].
+
+Theorem T_proof :
+  hasTableau OuterSkolemization {{ translate_EForm (Axiom0) ;; translate_EForm (ENeg T) }} subst.
+Proof.
+  exists \{ "X6_13" , "Y8_17" \}, \{ "skolem@X10@0", "skolem@Y4@1" \}.
+  unshelve eapply hasTableauNegAll with (sko := OuterSkolemization) (i := 0).
+  1, 2: shelve.
+  1: exact ((EFun "skolem@X10@0" [])).
+  2, 3: reflexivity.
+  1: { now esimpl. }
+  eapply hasTableauAll with (i := 2).
+  1: { reflexivity. }
+  1: { now esimpl. }
+  unshelve eapply hasTableauEx with (sko := OuterSkolemization) (i := 0).
+  1, 2: shelve.
+  1: exact ((EFun "skolem@Y4@1" [(EVar "X6_13")])).
+  2, 3: reflexivity.
+  1: { now esimpl. }
+  eapply hasTableauNegEx with (i := 3).
+  1: { reflexivity. }
+  1: { now esimpl. }
+  eapply hasTableauContr with (i := 2) (j := 0).
+  1: { reflexivity. }
+  1: { reflexivity. }
+  reflexivity.
+Qed.
