theories/Prelude/Atoms.v
@@ -8,9 +8,9 @@ From Tableaux Require Import Prelude.Sets.
 
 Class Atom :=
   { atom :> Type
-  ; eq_dec_atom : EqDec atom
+  ; eqb_atom : EqBool atom
   ; set_atom : set atom
-  ; isFresh : atom -> set_atom -> Prop }.
+  ; isFresh : atom -> set_atom -> bool }.
 Arguments set_atom : clear implicits.
 
 (** ** Some usual instantiations, hidden under an importable module. *)
@@ -20,13 +20,13 @@ Module AtomComputationalInstances.
 
   #[global] Canonical Structure nat_atom : Atom :=
     {| atom := nat
-    ;  eq_dec_atom := eq_dec_nat
+    ;  eqb_atom := eq_bool_nat
     ;  set_atom := SetOfNat
-    ;  isFresh := fun (x : nat) (S : SetOfNat) => ~(mem x S) |}.
+    ;  isFresh := fun (x : nat) (S : SetOfNat) => negb (mem x S) |}.
 
   #[global] Canonical Structure string_atom : Atom :=
     {| atom := string
-    ;  eq_dec_atom := eq_dec_string
+    ;  eqb_atom := eq_bool_string
     ;  set_atom := SetOfString
-    ;  isFresh := fun (x : string) (S : SetOfString) => ~(mem x S) |}.
+    ;  isFresh := fun (x : string) (S : SetOfString) => negb (mem x S) |}.
 End AtomComputationalInstances.
