theories/Prelude/Utils.v
@@ -1,5 +1,7 @@
 (** * Prelude.Utils: some utility functions / lemmas *)
 
+From Tableaux Require Import Init.
+
 Definition option_get {A : Type} (def : A) (x : option A) : A :=
   match x with
   | None => def
@@ -10,4 +12,11 @@ Definition bind {A B : Type} (x : option A) (f : A -> option B) : option B :=
   match x with
   | Some x => f x
   | None => None
+  end.
+
+Fixpoint forallb2 {A : Type} (P : A -> A -> bool) (l1 l2 : list A) : bool :=
+  match l1, l2 with
+  | [], [] => true
+  | x :: xs, y :: ys => P x y && forallb2 P xs ys
+  | _, _ => false
   end.
