devtools/run-tests.sh
@@ -1,0 +1,192 @@
+#!/bin/bash
+
+# Colors
+GREEN="$(tput setaf 2)"
+RED="$(tput setaf 1)"
+YELLOW="$(tput setaf 3)"
+BLUE="$(tput setaf 4)"
+SKY_BLUE="$(tput setaf 6)"
+RESET="$(tput sgr0)"
+
+# Functions for formatted messages
+ok() { echo "${GREEN}[OK]${RESET} $1"; }
+error() { echo "${RED}[ERROR]${RESET} $1"; }
+warn() { echo "${YELLOW}[WARN]${RESET} $1"; }
+info() { echo "${BLUE}[INFO]${RESET} $1"; }
+action() { echo "${SKY_BLUE}[ACTION]${RESET} $1"; }
+
+ROCQ_compile="rocq compile -Q ../theories Tableaux"
+
+# Check if ROCQ is installed
+if ! command -v rocq &>/dev/null; then
+  error "ROCQ is not installed."
+  info "Please follow the installation instructions in INSTALL.md"
+  exit 1
+fi
+
+# Check if TableauxRocq is compiled
+echo -n "From Tableaux Require Import All." > test_compile.v
+if $ROCQ_compile test_compile.v; then
+	rm -rf test_compile.v*
+	rm -rf test_compile.glob
+else
+	info "TableauxRocq has not been compiled. Compiling now..."
+	if cd .. && make -f RocqMakefile; then
+		ok "Succesfully compiled TableauxRocq."
+		cd devtools
+	else
+		error "Compilation of TableauxRocq has failed."
+		info "Please compile the TableauxRocq library."
+		exit 1
+	fi
+fi
+
+# Compile & bench all the files in a folder.
+# Enabling benches will fetch the previous version of TableauxRocq, compile
+# both version n times, and average out the compilation time.
+bench_n_compilations=10
+old_TR_name="TR_old"
+bench_results=$(pwd)/results
+repo_token=$1
+
+clone_and_make() {
+	if [[ ! -z "$repo_token" ]]; then
+		git fetch --unshallow
+	fi
+
+	current_commit=$(git rev-parse HEAD)
+	old_commit=$(git merge-base origin/master $current_commit)
+
+	action "Cloning TableauxRocq with commit $old_commit"
+	command="git clone git@github.com:jrosain/TableauxRocq.git"
+
+	if [[ ! -z "$repo_token" ]]; then
+		command="git clone https://x-access-token:$repo_token@github.com/jrosain/TableauxRocq.git"
+	fi
+
+	if $($command $old_TR_name); then
+		cd $old_TR_name
+		git config --add remote.origin.fetch "+refs/pull/*/head:refs/remotes/origin/pr/*"
+		git fetch --all
+		git checkout $old_commit
+
+		action "Compiling old TableauxRocq"
+		sh configure.sh
+		make -f RocqMakefile
+		cd devtools
+	else
+		error "Could not clone TableauxRocq"
+		exit 1
+	fi
+}
+
+compile_with_time() {
+	folder=$1
+	old_new=$2
+
+	TIMEFORMAT=%R
+
+	if [ -d $folder ]; then
+		for f in $(ls $folder/*.v); do
+			action "Checking that $f compiles..."
+			if $ROCQ_compile $f 2>/dev/null; then
+				action "Running benchs for $f"
+				test_results=$bench_results/$f.$old_new
+				mkdir -p $(dirname $test_results) && touch $test_results
+				for i in $(seq 1 $bench_n_compilations); do
+					out=$( { time rocq compile -Q ../theories Tableaux $f 2>/dev/null; } 2>&1 )
+					echo $out | tr , . >> $test_results
+				done
+			else
+				error "Could not compile $f."
+				info "Exiting with error."
+				exit 1
+			fi
+		done
+	fi
+
+	unset TIMEFORMAT
+}
+
+average() {
+	awk 'BEGIN { sum=0; count=0 } { sum += $1; count++ } END { print sum/count }' $1
+}
+
+make_results_summary() {
+	summary=$bench_results/summary
+	touch $summary
+	echo -e "File\t Diff.\t Avg. (new)\t Avg. (old)" >> $summary
+	for f in $(find $bench_results -type f -name "*.new"); do
+		f_name=${f%.new}
+		f_old=$f_name.old
+		if [ ! -f $f_old ]; then
+			avg=$(average $f)
+			# TODO: fix display + avg computation
+			echo -e "$(basename $f_name)\t -\t $avg sec.\t -" >> $summary
+		else
+			avg_new=average $f
+			avg_old=average $f_old
+			diff=$(( 100-(($avg_new*100)/$avg_old) ))
+			echo -e "$f_name\t $diff %\t $avg_new sec.\t $avg_old sec." >> $summary
+		fi
+	done
+
+	info "Benchs summary:"
+	column -t -s $'\t' $summary
+	echo ""
+}
+
+bench() {
+	folder=$1
+	current_folder=$(pwd)
+
+	action "Setup benches: cloning old TableauxRocq version"
+	mkdir $bench_results
+	clone_and_make
+
+	compile_with_time $folder "old"
+	cd $current_folder
+	compile_with_time $folder "new"
+	make_results_summary
+
+	action "Cleanup benches: remove old TableauxRocq version and temporary files"
+	rm -rf $old_TR_name
+	rm -rf $bench_results
+}
+
+compile_with_opt_bench() {
+	folder=$1
+	should_bench=$2
+
+	if [[ $should_bench = "bench" ]]; then
+		bench $folder
+	else
+		for f in $(ls $folder/*.v); do
+			action "ROCQ compile $f"
+			if $ROCQ_compile $f 2>/dev/null; then
+				ok "$f has successfully compiled."
+			else
+				error "Could not compile $f."
+				info "Exiting with error."
+				exit 1
+			fi
+		done
+	fi
+}
+
+compile() {
+	compile_with_opt_bench $1
+}
+
+compile_and_bench() {
+	compile_with_opt_bench $1 "bench"
+}
+
+# Sanity check: compile examples
+compile ../examples
+
+# Compile previous bugs
+compile tests
+
+# Run benches
+compile_and_bench tests/benchs
